adds typing for the asynchronous case study

theories/case_studies/asynchronous.v
@@ -34,23 +34,31 @@ Definition yield : val :=
           end)%V.
 
 Definition iter  : val:= 
-  (rec: "f" "g" "xs" := 
+  (Λ: rec: "f" "g" "xs" := 
     list-match: "xs" with
-        CONS "x" => "xxs" => "g" "x" ;; "f" "xxs"
+        CONS "x" => "xxs" => "g" "x" ;; "f" "g" "xxs"
       | NIL => #()
     end)%V.
 
+Definition next : val :=
+  (λ: "q" <>, list-match: "q" <!- NIL with
+              CONS "x" => "xs" => "q" <!- "xs" ;; "x" #()
+            | NIL => #()
+          end)%V.
+
+Definition add : val := 
+  (λ: "q" "f", "q" <!- CONS "f" ("q" <!- NIL) ;; #())%V.
+
+Definition resume_task : val := 
+  (λ: "add", Λ: λ: "v" "k", "add" (λ: <>, "k" "v"))%V.
+
 Definition runner : val :=
-  (λ: "main", 
+  (Λ: λ: "main", 
     let: "q" := ref NIL in  
 
-    let: "next" := 
-        (λ: <>, list-match: "q" <!- NIL with
-                    CONS "x" => "xs" => "q" <!- "xs" ;; "x" #()
-                  | NIL => #()
-                end)%E in
-    let: "add" := (λ: "f", "q" <!- CONS "f" ("q" <!- NIL))%E in
-    let: "resume_task" := (λ: "v" "k", "add" ("k" "v"))%E in
+    let: "add" := add "q" in
+    let: "next" := next "q" in
+    let: "resume_task" := resume_task "add" in
 
     let: "fulfill" := 
       (rec: "fulfill" <> := λ: "promise" "comp",   
@@ -60,30 +68,30 @@ Definition runner : val :=
               InjL "x" => 
                 (* async effect *) 
                 let: "new_prom" := ref (InjR NIL) in
-                "add" (λ: <>, "fulfill" #() "new_prom" "x") ;;
+                "add" (λ: <>, "fulfill" <_> "new_prom" "x") ;;
                 "k" (InjL "new_prom")
             | InjR "p" =>
                 (* await effect *) 
                 match: "p" <!- (InjR NIL) with
-                  InjL "v" => "p" <!- (InjL "v") ;; "k" "v"
-                | InjR "ks" => "p" <!- InjR (CONS "k" "ks") ;; "next" #()
+                  InjL "v" => "p" <!- (InjL "v") ;; "k" (InjR "v")
+                | InjR "ks" => "p" <!- InjR (CONS (λ: "v", "k" (InjR "v")) "ks") ;; "next" #()
                 end
             end
           )%E
         | return (λ: "x", 
-            let: "v" := "promise" <- InjR NIL in
+            let: "v" := "promise" <!- InjR NIL in
             match: "v" with
               InjL <> => impossible
             | InjR "ks" =>
-                "promise" <- InjL "v" ;;
-                iter ("resume_task" "v") "ks" ;;
+                "promise" <!- InjL "x" ;;
+                iter <_> ("resume_task" <_> "x") "ks" ;;
                 "next" #()
             end
           )%E
         end
       )%E in
       let: "pmain" := ref (InjR NIL) in
-      "fulfill" "pmain" "main" ;;
+      "fulfill" <_> "pmain" "main" ;;
       match: "pmain" <!- InjR NIL with
         InjL "v" => "v"
       | InjR <> => impossible
@@ -96,12 +104,22 @@ Section typing.
 
   Definition Queue := Refᶜ (List (() ⊸ ())).
 
-  Definition Status τ := τ + List (() ⊸ ()).
+  Definition Status τ := τ + List (τ ⊸ ()).
 
   Definition Promise τ := Refᶜ (Status τ).
 
   Definition asig := (∀μTS: θ, α, ( () -{ θ }-∘ '! α ) + Promise ('! α) ⇒ 
                                   Promise ('! α)       + '! α)%R. 
+
+  Definition iter_ty τ := (∀S: θ, (τ -{ θ }-> ()) → List τ -{ θ }-∘ ())%T.
+  
+  Definition next_ty := (() → ())%T.
+
+  Definition add_ty := ((() ⊸ ()) → ())%T.
+
+  Definition resume_task_ty := (∀T: α,, '! α → ('! α ⊸ ()) → ())%T.
+  
+  Definition runner_ty := (∀T: α,, (() -{ asig }-∘ '! α) → '! α)%T.
 
   Lemma impossible_typed τ :
     ⊢ ⊨ impossible : ⟨⟩ : τ.
@@ -174,4 +192,269 @@ Section typing.
       iApply impossible_typed.
   Qed.
 
+  Lemma iter_typed τ :
+    ⊢ ⊨ᵥ iter : iter_ty τ.
+  Proof.
+    iApply sem_typed_Sclosure. iIntros (ρ).
+    iApply sem_typed_sub_nil.
+    rewrite - {1} (app_nil_r []). 
+    iApply sem_typed_ufun; solve_sidecond. simpl.
+    rewrite - [[("g", _); ("f", _)]]app_nil_r. 
+    iApply sem_typed_afun; solve_sidecond. simpl.
+    set Γ₂ := [("g", τ -{ ρ }-> ());
+               ("f", ((τ -{ ρ }-> ()) → List τ -{ ρ }-∘ ())%T)].
+    iApply (sem_typed_match_list _ Γ₂); solve_sidecond.
+    - iApply sem_typed_sub_nil. rewrite - !/Γ₂.
+      iApply (sem_typed_var Γ₂).
+    - iApply sem_typed_sub_nil. 
+      do 2 iApply sem_typed_weaken.
+      iApply sem_typed_unit.
+    - iApply sem_typed_seq.
+      + iApply (sem_typed_app _ (("xxs", List τ) :: Γ₂) _ _ _ τ _ ()).
+        * iApply sem_typed_swap_second. 
+          iApply sem_typed_sub_nil.
+          iApply sem_typed_sub_ty; [apply ty_le_u2aarr|].
+          iApply sem_typed_contraction; solve_sidecond.
+          iApply sem_typed_var. 
+        * iApply sem_typed_sub_nil.
+          iApply sem_typed_var. 
+      + iApply sem_typed_swap_second. rewrite -/Γ₂.
+        do 2 (iApply sem_typed_app;
+          last (iApply sem_typed_sub_nil; iApply sem_typed_var)).
+        iApply sem_typed_sub_nil.
+        iApply sem_typed_sub_ty. 
+        { eapply ty_le_trans; [|apply ty_le_u2aarr].
+          apply ty_le_uarr. { apply sig_le_nil. }
+          apply ty_le_refl. apply ty_le_refl.
+          apply env_le_refl. apply env_le_refl. done. }
+        iApply sem_typed_var.
+  Qed.
+
+  Definition add_typed :
+    ⊢ ⊨ᵥ add : (Queue → add_ty).
+  Proof.
+    iIntros. rewrite /add_ty.
+    iApply sem_typed_closure; solve_sidecond. simpl.
+    set q := ("q", Queue). rewrite -(app_nil_r [q]).
+    iApply sem_typed_ufun; solve_sidecond. simpl.
+    set f := ("f", () ⊸ ()).
+    iApply (sem_typed_seq _ []); [|iApply sem_typed_unit].
+    iApply (sem_typed_replace_cpy _ [q]); [iApply sem_typed_var|].
+    iApply (sem_typed_cons _ [q;f]). 
+    { iApply sem_typed_swap_second. iApply sem_typed_var. }
+    iApply sem_typed_swap_second.
+    iApply sem_typed_replace_cpy; [|iApply sem_typed_nil].
+    iApply sem_typed_contraction; solve_sidecond.
+    iApply sem_typed_var.
+  Qed.
+
+  Definition next_typed :
+    ⊢ ⊨ᵥ next : (Queue → next_ty).
+  Proof.
+    iIntros. rewrite /next_ty.
+    iApply sem_typed_closure; solve_sidecond. simpl.
+    set q := ("q", Queue). rewrite -(app_nil_r [q]).
+    iApply sem_typed_ufun; solve_sidecond. simpl.
+    iApply (sem_typed_match_list _ [q]); solve_sidecond.
+    - iApply sem_typed_replace_cpy; [|iApply sem_typed_nil].
+      iApply sem_typed_contraction; solve_sidecond.
+      iApply sem_typed_var.
+    - iApply sem_typed_weaken. iApply sem_typed_unit.
+    - iApply sem_typed_swap_second.
+      iApply sem_typed_swap_third.
+      iApply sem_typed_swap_second.
+      set x := ("x", () ⊸ ()).
+      set xs := ("xs", List (() ⊸ ())).
+      rewrite -/q.
+      iApply (sem_typed_seq _ [x]). 
+      { iApply sem_typed_replace_cpy; iApply sem_typed_var. }
+      iApply sem_typed_app; [iApply sem_typed_var|iApply sem_typed_unit].
+  Qed.
+
+  Definition resume_task_typed :
+    ⊢ ⊨ᵥ resume_task : (add_ty → resume_task_ty).
+  Proof.
+    iIntros. rewrite /resume_task_ty.
+    iApply sem_typed_closure; solve_sidecond. simpl.
+    set add := ("add", add_ty)%T. rewrite -(app_nil_r [add]).
+    iApply sem_typed_TLam; solve_sidecond. iIntros (α).
+    rewrite -(app_nil_r [add]).
+    iApply sem_typed_ufun; solve_sidecond. simpl.
+    rewrite -(app_nil_r [("v", '! α); add]).
+    set v := ("v", '! α).
+    iApply sem_typed_ufun; solve_sidecond. simpl.
+    set k := ("k", '! α ⊸ ()).
+    iApply (sem_typed_app _ [add]). 
+    { iApply sem_typed_sub_ty; [apply ty_le_u2aarr|].
+      iApply sem_typed_var. }
+    replace ([k; v; add]) with ([k;v] ++ [add]) by done.
+    iApply sem_typed_afun; solve_sidecond. simpl.
+    iApply sem_typed_swap_second.
+    iApply sem_typed_app; iApply sem_typed_var.
+  Qed.
+
+  Definition runner_typed :
+    ⊢ ⊨ᵥ runner : runner_ty.
+  Proof.
+    iIntros. iApply sem_typed_Tclosure. iIntros (α).
+    rewrite - {1} (app_nil_r []).
+    iApply sem_typed_ufun; solve_sidecond. simpl.
+    set main := ("main", () -{ asig }-∘ '! α).
+    iApply (sem_typed_let _ [main]); solve_sidecond.
+    { iApply (sem_typed_alloc_cpy _ _ _ _ (List (() ⊸ ()))). 
+      iApply sem_typed_nil. }
+    iApply sem_typed_contraction; solve_sidecond.
+    set q := ("q", Queue).
+    iApply (sem_typed_let _ [q; main]); solve_sidecond.
+    { iApply sem_typed_app; [|iApply sem_typed_var].
+      iApply sem_typed_val. iApply add_typed. }
+    set add := ("add", add_ty).
+    iApply sem_typed_swap_second. 
+    iApply (sem_typed_let _ [add; main]); solve_sidecond. 
+    { rewrite /next. iApply sem_typed_app; [|iApply sem_typed_var].
+      iApply sem_typed_val. iApply next_typed. }
+    set next := ("next", next_ty).
+    iApply sem_typed_swap_second. 
+    iApply sem_typed_contraction; solve_sidecond.
+    iApply (sem_typed_let _ [add; next; main]); solve_sidecond.
+    { iApply sem_typed_app; [|iApply sem_typed_var].
+      iApply sem_typed_val. iApply resume_task_typed. }
+    set resume_task := ("resume_task", resume_task_ty).
+    rewrite -/next -/resume_task -/add.
+    iApply (sem_typed_let _ [main]); solve_sidecond.
+    - assert (Hrw : [resume_task;add;next;main] = [resume_task;add;next] ++ [main]) by done.
+      rewrite Hrw. clear Hrw.
+      iApply (sem_typed_ufun_poly_rec _ _ _ _ _ (λ β, Promise ('! β)) (λ _, ⟨⟩%R) (λ β, (() -{ asig }-∘ '! β) ⊸ ())); 
+        solve_sidecond. simpl.
+     iIntros (β) "/=". 
+     set promise := ("promise", Promise ('! β)).
+     set fulfill := ("fulfill", ∀T: β',, Promise ('! β') → (() -{ asig }-∘ '! β') ⊸ ()).
+     rewrite -(app_nil_r [promise;fulfill;resume_task;add;next]).
+     iApply sem_typed_afun; solve_sidecond. simpl.
+     set comp := ("comp", () -{ asig }-∘ '! β)%T.
+     replace ([comp; promise; fulfill; resume_task; add;next]) with
+             ([comp] ++ [promise; fulfill; resume_task; add;next]) by done.
+     set A := λ α θ, ( () -{ θ }-∘ '! α ) + Promise ('! α).
+     set B := (λ α (θ : sem_sig Σ), Promise ('! α) + '! α).
+     iApply (sem_typed_deep_try _ _ [] _ _ _ _ _ _ ⟨⟩%R A B); solve_sidecond.
+     { rewrite /A /Promise /Status. apply non_dep_fun_dist. by repeat f_equiv. }
+     { rewrite /B /Promise /Status. apply non_dep_fun_dist. by repeat f_equiv. }
+     + iApply sem_typed_app; [iApply sem_typed_sub_nil; iApply sem_typed_var|].
+       iApply sem_typed_sub_nil. iApply sem_typed_unit. 
+     + iIntros (β').
+       set k := ("k", B β' (∀μTS: θ, α0, A α0 θ ⇒ B α0 θ)%R ⊸ ()).
+       iApply sem_typed_swap_third. iApply sem_typed_weaken.
+       iApply sem_typed_swap_fourth. iApply sem_typed_weaken.
+       rewrite -/k -/fulfill.
+       iApply (sem_typed_match _ [k; fulfill; add; next]); solve_sidecond; [iApply sem_typed_var| |].
+       * simpl. set x := ("x", () -{ ∀μTS: θ, α0, A α0 θ ⇒ B α0 θ }-∘ '! β').
+         iApply (sem_typed_let _ [x; k; fulfill; add; next] _ _ _ _ (Promise ('! β'))); solve_sidecond.
+         { iApply sem_typed_alloc_cpy. iApply sem_typed_right_inj. iApply sem_typed_nil. }
+         set new_prom := ("new_prom", Promise ('! β')).
+         iApply (sem_typed_seq _ [new_prom; k; next]).
+         ** iApply (sem_typed_app _ [new_prom; k; add; next]).
+            { iApply sem_typed_swap_third.
+              iApply sem_typed_sub_ty; [apply ty_le_u2aarr|iApply sem_typed_var]. }
+            iApply sem_typed_swap_fourth. iApply sem_typed_swap_second.
+            iApply sem_typed_contraction; solve_sidecond.
+            do 2 iApply sem_typed_swap_fourth.
+            assert (Hrw : [fulfill; x; new_prom; new_prom; k; add; next] = 
+                          [fulfill; x; new_prom] ++ [new_prom; k; add; next]) by done.
+            rewrite Hrw. clear Hrw.
+            iApply sem_typed_afun; solve_sidecond. simpl.
+            do 2 (iApply sem_typed_swap_second; iApply sem_typed_app; [|iApply sem_typed_var]).
+            rewrite -/asig.
+            iApply sem_typed_sub_ty; [apply ty_le_u2aarr|]. 
+            set C := (λ β, Promise ('! β) → (() -{ asig }-∘ '! β) ⊸ ())%T.
+            rewrite -/(C β').
+            iApply sem_typed_TApp. iApply sem_typed_var.
+         ** iApply (sem_typed_app _ [k]); [iApply sem_typed_var|].
+            iApply sem_typed_swap_third. iApply sem_typed_weaken.
+            iApply sem_typed_left_inj. iApply sem_typed_var.
+      * simpl.
+        set p := ("p", Promise ('! β')).
+        do 2 (iApply sem_typed_swap_third; iApply sem_typed_weaken).
+        rewrite -/p -/k.
+        iApply (sem_typed_match _ [p;k;next]); solve_sidecond.
+        ** iApply sem_typed_replace_cpy; [iApply sem_typed_var|].
+           iApply sem_typed_contraction; solve_sidecond.
+           iApply sem_typed_right_inj. iApply sem_typed_nil.
+        ** simpl. set v := ("v", '! β').
+           iApply sem_typed_swap_fourth. iApply sem_typed_weaken.
+           iApply sem_typed_contraction; solve_sidecond.
+           iApply sem_typed_swap_third.
+           iApply sem_typed_swap_second.
+           iApply (sem_typed_seq _ [v; k]).
+           {  iApply sem_typed_replace_cpy; [iApply sem_typed_var|].
+             iApply sem_typed_left_inj. iApply sem_typed_var. }
+           iApply sem_typed_app; [iApply sem_typed_var|].
+           iApply sem_typed_right_inj. iApply sem_typed_var.
+        ** simpl. set ks := ("ks", List ('! β' ⊸ ())).
+           iApply (sem_typed_seq _ [next] _ _ _ (Status ('! β'))).
+           *** iApply sem_typed_swap_third. iApply (sem_typed_replace_cpy _ [p; next]).
+               { iApply sem_typed_var. }
+               iApply sem_typed_right_inj. 
+               rewrite /B /=. iApply sem_typed_swap_second.
+               iApply sem_typed_cons; [|iApply sem_typed_var]. 
+               assert (Hrw : [k; p; next] = [k] ++ [p;next]) by done.
+               rewrite Hrw. clear Hrw.
+               iApply sem_typed_afun; solve_sidecond. simpl.
+               iApply sem_typed_app; [iApply sem_typed_var|].
+               iApply sem_typed_right_inj. iApply sem_typed_var.
+           *** iApply sem_typed_app; [|iApply sem_typed_unit].
+               iApply sem_typed_sub_ty; [apply ty_le_u2aarr|iApply sem_typed_var].
+    + simpl. 
+      iApply sem_typed_swap_third. iApply sem_typed_weaken.
+      iApply sem_typed_swap_fourth; iApply sem_typed_weaken.
+      iApply sem_typed_swap_second.
+      set x := ("x", '!β). rewrite -/resume_task -/promise.
+      iApply (sem_typed_let _ [promise; x; resume_task; next]); solve_sidecond.
+      * iApply sem_typed_replace_cpy; [|iApply sem_typed_right_inj; iApply sem_typed_nil].
+        iApply sem_typed_contraction; solve_sidecond.
+        iApply sem_typed_var.
+      * set v := ("v", '! β + (List ('! β ⊸ ()))).
+        iApply (sem_typed_match _ [promise; x; resume_task; next]); solve_sidecond;
+          [iApply sem_typed_var| |].
+        { simpl. do 4 (iApply sem_typed_weaken). iApply impossible_typed. }
+        simpl. iApply sem_typed_swap_second. 
+        iApply sem_typed_swap_third. iApply sem_typed_contraction; solve_sidecond.
+        iApply sem_typed_swap_third. iApply sem_typed_swap_second.
+        set ks := ("ks", List ('! β ⊸ ())).
+        iApply (sem_typed_seq _ [x; ks; resume_task; next]).
+        ** iApply sem_typed_replace_cpy; [iApply sem_typed_var|].
+           iApply sem_typed_left_inj. iApply sem_typed_var.
+        ** iApply (sem_typed_seq _ [next]).
+           2: { iApply sem_typed_app; [|iApply sem_typed_unit].
+                iApply sem_typed_sub_ty; [apply ty_le_u2aarr|iApply sem_typed_var]. }
+           iApply sem_typed_swap_second.
+           iApply (sem_typed_app _ _ _ _ _ (List ('! β ⊸ ())) _ ()); [|iApply sem_typed_var].
+           iApply (sem_typed_app _ _ _ _ _ (('! β ⊸ ()) → ())%T).
+           2: { iApply sem_typed_app; [|iApply sem_typed_var]. 
+                iApply sem_typed_sub_ty; [apply ty_le_u2aarr|].
+                set C := λ β, ('! β → ('! β ⊸ ()) → ())%T. rewrite -/(C β).
+                iApply sem_typed_TApp. iApply sem_typed_var. }
+           iApply sem_typed_sub_ty; [apply ty_le_u2aarr|].
+           set C := (λ θ, (('! β ⊸ ()) -{ θ }-> ()) → List ('! β ⊸ ()) -{ θ }-∘ ())%T.
+           rewrite -/(C ⟨⟩%R).
+           iApply sem_typed_SApp. iApply sem_typed_val. iApply iter_typed.
+  - set fulfill := ("fulfill", ∀T: α,, Promise ('! α) → (() -{ asig }-∘ '! α) ⊸ ()).
+    iApply (sem_typed_let _ [fulfill; main]); solve_sidecond.
+    { iApply (sem_typed_alloc_cpy _ _ _ _ (Status ('! α))). 
+      iApply sem_typed_right_inj. iApply sem_typed_nil. }
+    set pmain := ("pmain", Refᶜ Status ('! α)).
+    iApply sem_typed_contraction; solve_sidecond.
+    iApply sem_typed_swap_third. iApply sem_typed_swap_second. iApply sem_typed_swap_fourth.
+    iApply (sem_typed_seq _ [pmain]).
+    + iApply (sem_typed_app _ _ _ _ _ _ _ ()); [|iApply sem_typed_var]. 
+      iApply sem_typed_app; [|iApply sem_typed_var]. 
+      iApply sem_typed_sub_ty; [apply ty_le_u2aarr|].
+      set C := (λ α, Promise ('! α) → (() -{ asig }-∘ '! α) ⊸ ())%T.
+      rewrite -/(C α).
+      iApply sem_typed_TApp. iApply sem_typed_var.
+    + iApply (sem_typed_match _ []); solve_sidecond; simpl; [|iApply sem_typed_var|].
+      { iApply sem_typed_replace_cpy; [iApply sem_typed_var|].
+        iApply sem_typed_right_inj. iApply sem_typed_nil. }
+      iApply impossible_typed. 
+  Qed.
+                  
 End typing.
