theories/lang/hazel.v
@@ -86,8 +86,8 @@ Notation NILV := (InjLV #()) (only parsing).
 Notation CONS x xs := (InjR (Pair x xs)) (only parsing).
 Notation CONSV x xs := (InjRV (PairV x xs)) (only parsing).
 
-Notation ListMatch e1 e2 x e3 := 
-  (Case (unfold: e1)%E (Lam BAnon e2) (Lam (BNamed x) (App (App e3 (Fst (Var x))) (Snd (Var x))))) (only parsing).
+Definition ListMatch e1 e2 x e3 := 
+  (Case (unfold: e1)%E (Lam BAnon e2) (Lam (BNamed x) (App (App e3 (Fst (Var x))) (Snd (Var x))))).
 Notation "'list-match:' e1 'with' 'CONS' x => xs => e3 | 'NIL' => e2 'end'" :=
   (ListMatch e1 e2%E x%binder (Lam x%binder (Lam xs%binder e3%E)))
   (e1, x, xs, e2, e1 at level 200,
